theories/utils.v
@@ -1,0 +1,248 @@
+(**************************************************************)
+(*   Copyright Dominique Larchey-Wendling [*]                 *)
+(*                                                            *)
+(*                             [*] Affiliation LORIA -- CNRS  *)
+(**************************************************************)
+(*      This file is distributed under the terms of the       *)
+(*        Mozilla Public License Version 2.0, MPL-2.0         *)
+(**************************************************************)
+
+From Coq Require Import List Relations Arith Lia Wellfounded Utf8.
+
+Import ListNotations.
+
+Set Implicit Arguments.
+
+(** Notations with global scope *)
+
+#[global] Notation "x ∈ l" := (In x l) (at level 70, no associativity, format "x  ∈  l").
+#[global] Notation ge R := (λ x y, x = y ∨ R y x).
+#[global] Notation "R ⁻¹" := (λ x y, R y x) (at level 1, left associativity, format "R ⁻¹").
+
+Arguments clos_trans {_}.
+Arguments clos_refl_trans {_}.
+Arguments transitive {_}.
+
+(** Tactics *)
+
+Tactic Notation "symm" :=
+  let H := fresh in
+  match goal with
+    |- _ = _ -> _ => intro H; symmetry in H; revert H
+  end.
+
+(** nat utils *)
+
+Fact lt_irrefl n : ¬ n < n.
+Proof. lia. Qed.
+
+Fact lt_trans a b c : a < b → b < c → a < c.
+Proof. lia. Qed.
+
+Section iter.
+
+  Variable (X : Type).
+
+  Implicit Type (f : X → X).
+
+  Definition iter f :=
+    fix loop n x := 
+      match n with
+      | 0   => x
+      | S n => loop n (f x)
+      end.
+
+  Fact iter_ext f g : (∀x, f x = g x) → ∀ n x, iter f n x = iter g n x.
+  Proof.
+    intros E n.
+    induction n as [ | n IHn ]; intro; simpl; auto. 
+    now rewrite E, IHn.
+  Qed.
+
+End iter.
+
+Arguments iter {_}.
+
+(** rel utils *)
+
+#[local] Hint Constructors clos_refl_trans clos_trans : core.
+
+Section clos_trans.
+
+  Variables (X : Type).
+
+  Implicit Type (R T : X → X → Prop).
+
+  Fact clos_trans_rev R x y : @clos_trans X R x y → clos_trans R⁻¹ y x. 
+  Proof. induction 1; eauto. Qed.
+  Fact clos_t_rt R x y z :
+       clos_trans R x y → clos_refl_trans R y z → clos_trans R x z.
+  Proof. induction 2; eauto. Qed.
+
+  Fact clos_trans_ge R : transitive R → ∀ x y, clos_trans (ge R) x y → ge R x y.
+  Proof. 
+    intros HR; red in HR.
+    induction 1 as [ ? ? [] | ? ? ? _ [] _ [] ]; subst; eauto.
+  Qed.
+
+  Fact clos_t_ge_rt R x y : clos_trans (ge R) x y → clos_refl_trans R y x.
+  Proof. induction 1 as [ ? ? [ <- | ] | ]; eauto. Qed.
+
+  Fact clos_trans_mono R T : 
+          (∀ x y, R x y → T x y)
+        → (∀ l m, clos_trans R l m → clos_trans T l m).
+  Proof. induction 2; eauto. Qed.
+
+  Hint Resolve clos_trans_rev : core.
+
+  Fact clos_trans_rev_iff R x y : clos_trans R⁻¹ x y ↔ (clos_trans R)⁻¹ x y.
+  Proof. split; auto. Qed.
+
+  Fact transitive_rev R : transitive R → transitive R⁻¹.
+  Proof. unfold transitive; eauto. Qed.
+
+End clos_trans.
+
+(** list utils *)
+
+#[local] Hint Resolve in_cons in_eq in_elt in_or_app : core.
+
+Fact rev_rect X (P : list X → Type) :
+      P [] → (∀ l x, P l → P (l++[x])) → ∀l, P l.
+Proof.
+  intros H1 H2 l; revert l P H1 H2.
+  induction l as [ | x l IH ]; intros P H1 H2; auto.
+  apply IH.
+  + apply (H2 []); auto.
+  + intros ? ? ?; now apply (H2 (_::_)).
+Qed.
+
+Inductive list_snoc_inv_shape X : list X → Type :=
+  | in_list_snoc_inv_shape l x : list_snoc_inv_shape (l++[x]).
+
+Fact list_snoc_inv X (l : list X) : l ≠ [] → list_snoc_inv_shape l.
+Proof.
+  destruct l as [ | l x ] using rev_rect.
+  + now intros [].
+  + constructor.
+Qed.
+
+Fact in_snoc_iff X (l : list X) x y : y ∈ l++[x] ↔ x = y ∨ y ∈ l.
+Proof. rewrite in_app_iff; simpl; tauto. Qed.
+
+Fact snoc_assoc X l (x y : X) : l++[x;y] = (l++[x])++[y].
+Proof. now rewrite <- app_assoc. Qed.
+
+Fact cons_inj {X} (x y : X) l m : x::l = y::m → x = y ∧ l = m.
+Proof. now inversion 1. Qed.
+
+Fact app_nil_inv {X} (l m : list X) : l++m = [] → l = [] ∧ m = [].
+Proof. revert l m; now intros [] []. Qed.
+
+Fact sg_eq_insert {X} (x y : X) l r : [x] = l++y::r → x = y ∧ l = [] ∧ r = [].
+Proof. destruct l as [ | ? [] ]; inversion 1; auto. Qed.
+
+Fact list_split {X} (l₁ l₂ r₁ r₂ : list X) :
+    l₁++r₁ = l₂++r₂
+  → ∃m, l₁++m = l₂ ∧ r₁ = m++r₂
+     ∨  l₁ = l₂++m ∧ m++r₁ = r₂.
+Proof.
+  revert l₂; induction l₁ as [ | x l1 IH ]; intros [ | y l2 ]; simpl.
+  + exists []; auto.
+  + intros ->; eauto.
+  + intros <-; eauto.
+  + injection 1; intros (m & [ [] | [] ])%IH <-; subst; eauto.
+Qed.
+
+Fact list_split_cons {X} (l₁ l₂ r₁ r₂ : list X) x :
+    l₁++r₁ = l₂++[x]++r₂
+  → ∃m, l₁++m = l₂ ∧ r₁ = m++[x]++r₂
+     ∨  l₁ = l₂++[x]++m ∧ m++r₁ = r₂.
+Proof.
+  intros (m & [ [H1 H2] | [H1 H2] ])%list_split; subst; eauto.
+  destruct m as [ | y m ]; simpl in H2.
+  + subst; exists []; rewrite !app_nil_r; auto.
+  + inversion H2; subst; exists m; auto.
+Qed. 
+
+Fact list_split_cons2 {X} (l₁ l₂ r₁ r₂ : list X) x y :
+    l₁++[x]++r₁ = l₂++[y]++r₂
+  → l₁ = l₂ ∧ x = y ∧ r₁ = r₂
+  ∨ ∃m, l₁++[x]++m = l₂ ∧ r₁ = m++[y]++r₂
+     ∨  l₁ = l₂++[y]++m ∧ m++[x]++r₁ = r₂.
+Proof.
+  intros (m & [ [H1 H2] | [H1 H2] ])%list_split; subst.
+  + destruct m as [ | z m ]; simpl in H2.
+    * inversion H2; subst y r₂.
+      rewrite app_nil_r; auto.
+    * inversion H2; subst z r₁.
+      right; exists m; auto.
+  + destruct m as [ | z m ]; simpl in H2.
+    * inversion H2; subst y r₂.
+      rewrite app_nil_r; auto.
+    * inversion H2; subst z r₂.
+      right; exists m; auto.
+Qed.
+
+Fact list_nil_choose X (l : list X) : {l = []} + {l ≠ []}.
+Proof. destruct l; eauto; now right. Qed.
+
+Fact list_fall_choose X (P Q : X → Prop) l :
+        (∀x, x ∈ l → {P x} + {Q x})
+      → { x | x ∈ l ∧ P x } + { ∀x, x ∈ l → Q x }.
+Proof.
+  induction l as [ | x l IHl ]; intros Hl.
+  + now right.
+  + destruct (Hl x); eauto.
+    destruct IHl as [ (? & []) | ]; eauto.
+    right; intros ? [<- |]; eauto.
+Qed.
+
+(** Squashing a decidable predidate into an equivalent
+    one that has unique proofs *)
+
+Section squash.
+
+  (* Squashing map a (strongly) decidable predicate into
+     an equivalent proof irrelevant one *)
+
+  Variables (P : Prop) (d : {P}+{¬P}).
+
+  Definition squash := if d then True else False.
+
+  Fact squash_iff : squash ↔ P.
+  Proof. unfold squash; destruct d; tauto. Qed.
+
+  Fact squash_pirr : ∀ p1 p2 : squash, p1 = p2.
+  Proof. unfold squash; destruct d; now intros [] []. Qed.
+
+End squash.
+
+(** Acc utils, morphims *)
+
+#[local] Hint Resolve Acc_inv Acc_intro : core.
+
+Fact Acc_irrefl X (R : X → X → Prop) x : Acc R x → ~ R x x.
+Proof. induction 1 as [ x _ IH ]; intros H; exact (IH _ H H). Qed.
+
+Section wf_rel_morph.
+
+  Variables (X Y : Type) (R : X → X → Prop) (T : Y → Y → Prop)
+            (f : X → Y → Prop)
+            (f_surj : ∀y, ∃x, f x y)
+            (f_morph : ∀ x₁ x₂ y₁ y₂, f x₁ y₁ → f x₂ y₂ → T y₁ y₂ → R x₁ x₂).
+
+  Theorem Acc_rel_morph x y : f x y → Acc R x → Acc T y.
+  Proof.
+    intros H1 H2; revert H2 y H1.
+    induction 1 as [ x _ IH ]; intros y ?.
+    constructor; intros z ?.
+    destruct (f_surj z); eauto.
+  Qed.
+
+  Hint Resolve Acc_rel_morph : core.
+
+  Corollary wf_rel_morph : well_founded R → well_founded T.
+  Proof. intros ? y; destruct (f_surj y); eauto. Qed.
+
+End wf_rel_morph.
